specs/Spec.Agile.CTR.fst
@@ -8,47 +8,31 @@ open Spec.Agile.Cipher
 
 #reset-options "--z3rlimit 20 --max_fuel 0 --max_ifuel 1"
 
-let state (a:cipher_alg) =
+// So that clients don't need to open both modules
+include Spec.Agile.Cipher
+
+let key_length (a: cipher_alg) =
   match a with
-  | AES128 | AES256 -> Spec.AES.aes_ctr_state (aes_alg_of_alg a)
-  | CHACHA20 -> Spec.Chacha20.state
+  | AES128 | AES256 -> Spec.AES.key_size (aes_alg_of_alg a)
+  | CHACHA20 -> Spec.Chacha20.size_key
 
-val process_block:
-  a:cipher_alg ->
-  st0:state a ->
-  c:size_nat {c <= counter_max a} ->
-  plain:lbytes (block_len a) ->
-  Tot (lbytes (block_len a))
-let process_block a st0 c plain =
-  let st = add_counter a st0 c in
-  let k = key_block a st in
-  let c = map2 ( ^. ) plain k in
-  c
+let key (a: cipher_alg) =
+  match a with
+  | AES128 | AES256 -> Spec.AES.aes_key (aes_alg_of_alg a)
+  | CHACHA20 -> Spec.Chacha20.key
 
-val process_last:
-  a:cipher_alg ->
-  st0:state a ->
-  c:size_nat {c <= counter_max a} ->
-  len:size_nat{len < block_len a} ->
-  plain:lbytes len ->
-  Tot (lbytes len)
-let process_last a st0 c len plain =
- let last = create (block_len a) (u8 0) in
- let last = update_sub last 0 len plain in
- let cipher = process_block a st0 c last in
- sub cipher 0 len
+let expand (a: cipher_alg) (k: key a): xkey a =
+  match a with
+  | AES128 | AES256 -> Spec.AES.aes_key_expansion (aes_alg_of_alg a) k
+  | CHACHA20 -> k
 
 val counter_mode:
   a:cipher_alg ->
-  k:lbytes (key_len a) ->
-  n_len:(nonce_len a) ->
-  n:lbytes n_len ->
-  c:size_nat{c <= counter_max a} ->
-  len: size_nat{c + (len / block_len a) <= counter_max a}  ->
-  plain:lbytes len  ->
-  Tot (lbytes len)
-let counter_mode a key n_len nonce counter len plain =
-  let st0 = init a key n_len nonce counter in
-  map_blocks (block_len a) plain
-    (process_block a st0)
-    (process_last a st0)
+  k:key a ->
+  n:nonce a ->
+  plain:bytes { length plain <= max_size_t } ->
+  Tot (cipher:bytes { length cipher = length plain })
+let counter_mode a k n plain =
+  let xk = expand a k in
+  let stream = ctr_stream a xk n (length plain) in
+  map2 ( ^. ) (plain <: lbytes (length plain)) (stream <: lbytes (length plain))
