specs/Spec.AEAD.fsti
@@ -75,7 +75,7 @@ let ekv_length: supported_alg -> nat =
 let max_length: supported_alg -> nat =
   function
   | CHACHA20_POLY1305 -> pow2 32 - 1 - 16
-  | AES128_GCM | AES256_GCM -> pow2 32 - 1 
+  | AES128_GCM | AES256_GCM -> pow2 32 - 1
 
 // Proudly defining this type abbreviation for the tenth time in HACL*!
 let lbytes (l:nat) = b:Seq.seq UInt8.t { Seq.length b = l }
