specs/Spec.Agile.Cipher.fsti
@@ -1,0 +1,82 @@
+module Spec.Agile.Cipher
+
+open FStar.Mul
+open Lib.IntTypes
+open Lib.Sequence
+open Lib.ByteSequence
+
+#reset-options "--z3rlimit 20 --max_fuel 0 --max_ifuel 1"
+
+/// This module is concerned with defining an agile stream cipher, i.e. a
+/// function that given: a suitably extended key; an iv (nonce); a counter,
+/// produces a fresh block.
+///
+/// TODO: share definitions with Spec.AEAD, in particular definitions of nonce,
+/// key, key expansion, etc.
+
+type cipher_alg =
+  | AES128
+  | AES256
+  | CHACHA20
+
+/// The AES spec itself is agile; this is the same nested agility technique used
+/// for SHA2 vs. MD.
+let aes_alg_of_alg (a: cipher_alg { a = AES128 \/ a = AES256 }) =
+  match a with
+  | AES128 -> Spec.AES.AES128
+  | AES256 -> Spec.AES.AES256
+
+/// Algorithms may (AES) or may not (Chacha) require a preliminary round of key expansion.
+let xkey (a: cipher_alg) =
+  match a with
+  | AES128 | AES256 -> Spec.AES.aes_xkey (aes_alg_of_alg a)
+  | CHACHA20 -> Spec.Chacha20.key
+
+/// Trying to enforce conventions: lengths for nats (spec); len for machine
+/// integers (runtime).
+let block_length (a:cipher_alg) =
+  match a with
+  | AES128 | AES256 -> 16
+  | CHACHA20 -> 64
+
+/// Type abbreviations.
+let block a = lbytes (block_length a)
+
+let ctr = size_nat
+
+let nonce_bound (a: cipher_alg) (n_len: nat): Type0 =
+  match a with
+  | AES128 | AES256 -> n_len <= block_length a
+  | CHACHA20 -> n_len == 12
+
+let nonce a = b:bytes { nonce_bound a (length b) }
+
+val ctr_block (a: cipher_alg) (k: xkey a) (iv: nonce a) (c: ctr): block a
+
+/// A stream of pseudo-random bytes, starting from counter zero. The length is
+/// artificially constrained to be < 2^32.
+let ctr_stream (a: cipher_alg) (k: xkey a) (iv: nonce a) (len: size_nat):
+  b:bytes { length b = len }
+=
+  // JP: useful? be overconservative and always do + 1? would necessitate a
+  // little bit of reasoning on the implementation side, perhaps better to have
+  // a tighter bound here
+  let n_blocks: n:nat { n * block_length a >= len } =
+    if len % block_length a = 0 then
+      len / block_length a
+    else
+      len / block_length a + 1
+  in
+  let (), blocks = generate_blocks
+    (block_length a)
+    max_size_t
+    n_blocks
+    (fun _ -> unit) // extra cruft; no accumulator here
+    (fun i _ -> (), ctr_block a k iv i )
+    ()
+  in
+  Seq.slice blocks 0 len
+
+/// Possible addition: ctr_stream_n, which generates ``len`` bytes starting from
+/// counter ``n`` (or, possibly, from bytes ``n``). I don't think it's necessary
+/// to have that one to properly specify ``EverCrypt.CTR``.
